src/DatalogCompilers/StringGridCompiler.v
@@ -38,8 +38,8 @@ Definition make_layout_map
 Definition compile_program
     (program        : list rule)
     (layout         : list (node_id * list nat))
-    (fact_producers : fact_locations (node_id := node_id))
-    (fact_consumers : fact_locations (node_id := node_id))
+    (fact_producers : rel_locs_map)
+    (fact_consumers : rel_locs_map)
     (topo_dims      : GridGraph.Dimensions)
     : _ :=
   compile
@@ -67,8 +67,8 @@ Definition compile_program
 Definition compile_program_rel_ids
     (program        : list rule)
     (layout         : list (node_id * list nat))
-    (fact_producers : fact_locations (node_id := node_id))
-    (fact_consumers : fact_locations (node_id := node_id))
+    (fact_producers : rel_locs_map)
+    (fact_consumers : rel_locs_map)
     : _ :=
   compile_rel_ids
     (node_id            := node_id)
